RedisProof/ProofStructured/Layer2/RefineRel.v
@@ -1,4 +1,0 @@
-Require Import CommonDeps.
-Require Import DataTypes.
-
-Definition refrel (hst: RData) (lst: RData) : Prop := hst = lst.
