RedisProof/Finished/ProofLayer1/.CachedSpec/BottomSpec.v
@@ -1,0 +1,43 @@
+Definition abort_spec (st: RData) : (option RData) :=
+  (Some st).
+
+Definition timeInMilliseconds_spec (st: RData) : (option (Z * RData)) :=
+  (Some ((st.(time)), (st.[time] :< ((st.(time)) + (10))))).
+
+Definition printf_spec (p: Ptr) (st: RData) : (option (Z * RData)) :=
+  (Some (1, st)).
+
+Definition zmalloc_spec (v_size: Z) (st: RData) : (option (Ptr * RData)) :=
+  let offset := ((st.(memory)).(offset)) in
+  (Some ((mkPtr "memory" offset), (st.[memory].[offset] :< (offset + (v_size))))).
+
+Definition _dictPanic_spec (p: Ptr) (st: RData) : (option RData) :=
+  (Some st).
+
+Definition zfree_spec (p: Ptr) (st: RData) : (option RData) :=
+  if ((p.(pbase)) =s ("memory"))
+  then (
+    let n_data := (((st.(memory)).(data)) # (p.(poffset)) == None) in
+    (Some (st.[memory].[data] :< n_data)))
+  else (Some st).
+
+Definition random_spec (st: RData) : (option (Z * RData)) :=
+  (Some (0, st)).
+
+Definition llvm_memset_p0i8_i64_spec (p: Ptr) (v: Z) (sz: Z) (b: bool) (st: RData) : (option RData) :=
+  rely (((p.(pbase)) = ("memory")));
+  let n_data := (((st.(memory)).(data)) # (p.(poffset)) == (Some v)) in
+  (Some (st.[memory].[data] :< n_data)).
+
+Definition llvm_memcpy_p0i8_p0i8_i64_spec (dst: Ptr) (src: Ptr) (sz: Z) (b: bool) (st: RData) : (option RData) :=
+  (Some st).
+
+Definition strcmp_spec (p1: Ptr) (p2: Ptr) (st: RData) : (option (Z * RData)) :=
+  (Some (0, st)).
+
+Definition strlen_spec (p: Ptr) (st: RData) : (option (Z * RData)) :=
+  (Some (0, st)).
+
+Definition _dictExpandIfNeeded_spec (p: Ptr) (st: RData) : (option (Z * RData)) :=
+  (Some (0, st)).
+
