RedisProof/Finished/ProofLayer1/.CachedSpec/Layer1Spec.v
@@ -1,0 +1,35 @@
+Definition _dictFree_spec (ptr: Ptr) (st: RData) : (option RData) :=
+  if ((ptr.(pbase)) =s ("memory"))
+  then (Some (st.[memory].[data] :< (((st.(memory)).(data)) # (ptr.(poffset)) == None)))
+  else (Some st).
+
+Definition _dictAlloc_spec (size: Z) (st: RData) : (option (Ptr * RData)) :=
+  let offset := ((st.(memory)).(offset)) in
+  (Some ((mkPtr "memory" offset), (st.[memory].[offset] :< (offset + (size))))).
+
+Definition _dictReset_spec (ht: Ptr) (st: RData) : (option RData) :=
+  if ((ht.(pbase)) =s ("memory"))
+  then (
+    (Some (st.[memory].[data] :<
+      ((((((st.(memory)).(data)) # (ht.(poffset)) == (Some 0)) # ((ht.(poffset)) + (8)) == (Some 0)) # ((ht.(poffset)) + (16)) == (Some 0)) #
+        ((ht.(poffset)) + (24)) ==
+        (Some 0)))))
+  else (
+    if ((ht.(pbase)) =s ("dict_can_resize"))
+    then (Some (st.[dict_can_resize] :< 0))
+    else (Some bad_st)).
+
+Fixpoint _dictNextPower_loop_0 (size: Z) (i_0: Z) (arg_dummy0: Z) (arg_dummy1: Z) (st: RData) : (option (Z * Z * Z * Z * RData)) :=
+  if ((i_0 - (size)) >=? (0))
+  then (Some (size, i_0, i_0, 0, st))
+  else (_dictNextPower_loop_0 size (i_0 * (2)) arg_dummy0 arg_dummy1 st).
+
+Definition _dictNextPower_spec (size: Z) (st: RData) : (option (Z * RData)) :=
+  if (size >=? (9223372036854775807))
+  then (Some (9223372036854775807, st))
+  else (
+    match ((_dictNextPower_loop_0 size 4 0 0 st)) with
+    | (Some (size_after, i_0_after, i_0, v_0, st_0)) => (Some (i_0, st_0))
+    | None => None
+    end).
+
