RedisProof/Finished/ProofLayer1/DataTypes.v
@@ -1,0 +1,63 @@
+Require Import CommonDeps.
+
+Local Open Scope Z_scope.
+
+Inductive nat: Type :=
+ | O 
+ | S (pred: nat).
+
+
+Record Memory :=
+  mkMemory {
+    offset: Z;
+    data: (ZMap.t (option Z));
+}.
+
+
+Record RData :=
+  mkRData {
+    memory: Memory;
+    time: Z;
+    dict_can_resize: Z;
+}.
+
+
+Definition update_Memory_offset(_a: Memory) _b :=
+  mkMemory _b (_a.(data)).
+Notation "_a '.[offset]' ':<' _b" := (update_Memory_offset _a _b) (at level 1).
+
+Definition update_Memory_data(_a: Memory) _b :=
+  mkMemory (_a.(offset)) _b.
+Notation "_a '.[data]' ':<' _b" := (update_Memory_data _a _b) (at level 1).
+
+Definition update_RData_memory(_a: RData) _b :=
+  mkRData _b (_a.(time)) (_a.(dict_can_resize)).
+Notation "_a '.[memory]' ':<' _b" := (update_RData_memory _a _b) (at level 1).
+
+Definition update_RData_time(_a: RData) _b :=
+  mkRData (_a.(memory)) _b (_a.(dict_can_resize)).
+Notation "_a '.[time]' ':<' _b" := (update_RData_time _a _b) (at level 1).
+
+Definition update_RData_dict_can_resize(_a: RData) _b :=
+  mkRData (_a.(memory)) (_a.(time)) _b.
+Notation "_a '.[dict_can_resize]' ':<' _b" := (update_RData_dict_can_resize _a _b) (at level 1).
+
+Definition update_RData_memory_offset(_a: RData) _b :=
+  update_RData_memory _a ((_a.(memory)).[offset] :< _b).
+Notation "_a '.[memory].[offset]' ':<' _b" := (update_RData_memory_offset _a _b) (at level 1).
+
+Definition update_RData_memory_data(_a: RData) _b :=
+  update_RData_memory _a ((_a.(memory)).[data] :< _b).
+Notation "_a '.[memory].[data]' ':<' _b" := (update_RData_memory_data _a _b) (at level 1).
+
+#[global] Hint Unfold
+  update_Memory_offset
+  update_Memory_data
+  update_RData_memory
+  update_RData_time
+  update_RData_dict_can_resize
+  update_RData_memory_offset
+  update_RData_memory_data
+  : update_RData.
+
+Ltac simpl_RData := autounfold with update_RData; simpl.
