RedisProof/Finished/ProofLayer1/Layer1/Spec.v
@@ -1,0 +1,74 @@
+Require Import CommonDeps.
+Require Import DataTypes.
+Require Import GlobalDefs.
+
+Local Open Scope string_scope.
+Local Open Scope Z_scope.
+
+(* loop fix *)
+Require Import Coq.Program.Wf.
+Require Import Coq.ZArith.ZArith.
+
+Section Layer1_Spec.
+
+  Context `{int_ptr: IntPtrCast}.
+
+  Definition _dictFree_spec (ptr: Ptr) (st: RData) : (option RData) :=
+    if ((ptr.(pbase)) =s ("memory"))
+    then (Some (st.[memory].[data] :< (((st.(memory)).(data)) # (ptr.(poffset)) == None)))
+    else (Some st).
+
+  Definition _dictAlloc_spec (size: Z) (st: RData) : (option (Ptr * RData)) :=
+    let offset := ((st.(memory)).(offset)) in
+    (Some ((mkPtr "memory" offset), (st.[memory].[offset] :< (offset + (size))))).
+
+  Definition _dictReset_spec (ht: Ptr) (st: RData) : (option RData) :=
+    if ((ht.(pbase)) =s ("memory"))
+    then (
+      (Some (st.[memory].[data] :<
+        ((((((st.(memory)).(data)) # (ht.(poffset)) == (Some 0)) # ((ht.(poffset)) + (8)) == (Some 0)) # ((ht.(poffset)) + (16)) == (Some 0)) #
+          ((ht.(poffset)) + (24)) ==
+          (Some 0)))))
+    else (
+      if ((ht.(pbase)) =s ("dict_can_resize"))
+      then (Some (st.[dict_can_resize] :< 0))
+      else (Some bad_st)).
+
+  (* Fixpoint _dictNextPower_loop_0 (size: Z) (i_0: Z) (arg_dummy0: Z) (arg_dummy1: Z) (st: RData) : (option (Z * Z * Z * Z * RData)) :=
+    if ((i_0 - (size)) >=? (0))
+    then (Some (size, i_0, i_0, 0, st))
+    else (_dictNextPower_loop_0 size (i_0 * (2)) arg_dummy0 arg_dummy1 st). *)
+
+  Program Fixpoint _dictNextPower_loop_0
+        (size i_0 arg_dummy0 arg_dummy1 : Z)
+        (st : RData)
+  {measure (Z.to_nat (size - i_0))}
+  : option (Z * Z * Z * Z * RData) :=
+      relyp (i_0 > 0);
+      match i_0 >=d size with
+      | left _   => Some (size, i_0, i_0, 0, st)
+      | right Hlt => _dictNextPower_loop_0 size (i_0 * 2) arg_dummy0 arg_dummy1 st
+      end.
+  Next Obligation.
+    (* Goal: Z.to_nat (size - i_0 * 2) < Z.to_nat (size - i_0)
+      Context: ~ i_0 <= 0       => i_0 > 0
+               ~ i_0 >= size    => i_0 < size  *)
+    lia.
+  Defined.
+
+  Definition _dictNextPower_spec (size: Z) (st: RData) : (option (Z * RData)) :=
+    if (size >=? (9223372036854775807))
+    then (Some (9223372036854775807, st))
+    else (
+      match ((_dictNextPower_loop_0 size 4 0 0 st)) with
+      | (Some (size_after, i_0_after, i_0, v_0, st_0)) => (Some (i_0, st_0))
+      | None => None
+      end).
+
+End Layer1_Spec.
+
+#[global] Hint Unfold _dictFree_spec: spec.
+#[global] Hint Unfold _dictAlloc_spec: spec.
+#[global] Hint Unfold _dictReset_spec: spec.
+#[global] Hint Unfold _dictNextPower_loop_0: spec.
+#[global] Hint Unfold _dictNextPower_spec: spec.
