RedisProof/Finished/ProofLayer1/Layer1/_dictAlloc/RefProof.v
@@ -1,0 +1,32 @@
+Require Import Bottom.Layer.
+Require Import Bottom.Spec.
+Require Import CommonDeps.
+Require Import DataTypes.
+Require Import Layer1.Layer.
+Require Import Layer1.RefineRel.
+Require Import Layer1.Spec.
+Require Import Layer1._dictAlloc.LowSpec.
+Require Import GlobalDefs.
+Require Import LayerSem.Libs.Zutils.div_mod_to_equations.
+
+Local Open Scope string_scope.
+Local Open Scope Z_scope.
+Local Opaque Z.add Z.mul Z.div Z.sub Z.land Z.lor Z.lxor Z.shiftl Z.shiftr Z.quot Z.rem.
+
+Section DictPrim__dictAlloc_RefProof.
+
+  Context `{int_ptr: IntPtrCast}.
+
+  Lemma f__dictAlloc_refine:
+    forall v_size lst hst hst' res
+           (Hrel: refrel hst lst)
+           (Hspec: _dictAlloc_spec v_size hst = Some (res, hst')),
+      exists lst', _dictAlloc_spec_low v_size lst = Some (res, lst') /\ refrel hst' lst'.
+    Proof.
+      intros; inv Hrel.
+      autounfold with spec in *; autounfold with sem in *; simpl in *.
+      destruct_spec Hspec; repeat (solve_refproof; repeat rewrite annotation_eq);
+        repeat eexists; try unfold refrel; solve_equality.
+    Qed.
+
+End DictPrim__dictAlloc_RefProof.
