RedisProof/Finished/ProofLayer1/Layer1/_dictFree/LowSpec.v
@@ -1,0 +1,19 @@
+Require Import Bottom.Spec.
+Require Import CommonDeps.
+Require Import DataTypes.
+Require Import GlobalDefs.
+
+Local Open Scope string_scope.
+Local Open Scope Z_scope.
+
+Section Layer1__dictFree_LowSpec.
+
+  Context `{int_ptr: IntPtrCast}.
+
+  Definition _dictFree_spec_low (ptr: Ptr) (st: RData) : (option RData) :=
+    when st_0 == ((zfree_spec ptr st));
+    (Some st_0).
+
+End Layer1__dictFree_LowSpec.
+
+#[global] Hint Unfold _dictFree_spec_low: spec.
