RedisProof/ProofStructured/.CachedSpec/Layer1Spec.v
@@ -1,9 +1,0 @@
-Definition _dictReset_spec (ht: Ptr) (st: RData) : (option RData) :=
-  if ((ht.(pbase)) =s ("dictht"))
-  then (
-    (Some (st.[dicthtStore].[data] :<
-      ((((((st.(dicthtStore)).(data)) # (ht.(poffset)) == (Some 0)) # ((ht.(poffset)) + (8)) == (Some 0)) # ((ht.(poffset)) + (16)) == (Some 0)) #
-        ((ht.(poffset)) + (24)) ==
-        (Some 0)))))
-  else (Some bad_st).
-
